GDPRhealthcare.thy
@@ -1,137 +1,169 @@
-theory HealthcareExample
-imports Insider 
+theory GDPRhealthcare
+imports Infrastructure
 begin
 
-locale scenarioHealthcare = 
-fixes healthcare_actors :: "identity set"
-defines healthcare_actors_def: "healthcare_actors \<equiv> {''Patient''}"
+locale scenarioGDPR = 
+fixes gdpr_actors :: "identity set"
+defines gdpr_actors_def: "gdpr_actors \<equiv> {''Patient'', ''Doctor''}"
 
-fixes hc_locations :: "location set"
-defines hc_locations_def: "hc_locations \<equiv> 
+fixes gdpr_locations :: "location set"
+defines gdpr_locations_def: "gdpr_locations \<equiv> 
           {Location 0, Location 1, Location 2, Location 3}"
 
 fixes sphone :: "location"
 defines sphone_def: "sphone \<equiv> Location 0"
-fixes room :: "location"
-defines room_def: "room \<equiv> Location 1"
-fixes bankapp :: "location"
-defines bankapp_def: "bankapp \<equiv> Location 2"
-fixes healthapp :: "location"
-defines healthapp_def: "healthapp \<equiv> Location 3"
+fixes home :: "location"
+defines home_def: "home \<equiv> Location 1"
+fixes hospital :: "location"
+defines hospital_def: "hospital \<equiv> Location 2"
+fixes cloud :: "location"
+defines cloud_def: "cloud \<equiv> Location 3"
 
 fixes global_policy :: "[infrastructure, identity] \<Rightarrow> bool"
-defines global_policy_def: "global_policy I a \<equiv> a \<noteq> ''Patient'' 
-                 \<longrightarrow> \<not>(enables I bankapp (Actor a) eval)"
+defines global_policy_def: "global_policy I a \<equiv> a \<noteq> ''Doctor'' 
+                 \<longrightarrow> \<not>(enables I hospital (Actor a) eval)"
 
+  
+  
 fixes ex_creds :: "actor \<Rightarrow> (string set * string set)"
 defines ex_creds_def: "ex_creds \<equiv> (\<lambda> x. if x = Actor ''Patient'' then 
                          ({''PIN'',''skey''}, {}) else 
-                            (if x = Actor ''Carer'' then
+                            (if x = Actor ''Doctor'' then
                                 ({''PIN''},{}) else ({},{})))"
 
 fixes ex_creds' :: "actor \<Rightarrow> (string set * string set)"
 defines ex_creds'_def: "ex_creds' \<equiv> (\<lambda> x. if x = Actor ''Patient'' then 
                          ({''PIN'',''skey''}, {}) else 
-                            (if x = Actor ''Carer'' then
+                            (if x = Actor ''Doctor'' then
                                 ({''PIN'',''skey''}, {}) else ({},{})))"
 
-fixes ex_locs :: "location \<Rightarrow> string set"
-defines "ex_locs \<equiv> (\<lambda> x.  {})"
+fixes ex_locs :: "location \<Rightarrow> string * acond"
+defines "ex_locs \<equiv> (\<lambda> x.  (''free'',{((Actor ''Patient'',{Actor ''Doctor''}),42)}))"
 
   
 fixes ex_graph :: "igraph"
 defines ex_graph_def: "ex_graph \<equiv> Lgraph 
-     {(room, sphone), (sphone, healthapp), (sphone,bankapp)}
-     (\<lambda> x. if x = room then {''Patient'', ''Carer''} else {}) 
+     {(home, cloud), (sphone, cloud), (cloud,hospital)}
+     (\<lambda> x. if x = home then {''Patient''} else 
+           (if x = hospital then {''Doctor''} else {})) 
      ex_creds ex_locs"
   
 fixes ex_graph' :: "igraph"
 defines ex_graph'_def: "ex_graph' \<equiv> Lgraph 
-     {(room, sphone), (sphone, healthapp), (sphone,bankapp)}
-     (\<lambda> x. if x = room then {''Patient'', ''Carer''} else {}) 
+     {(home, cloud), (sphone, cloud), (cloud,hospital)}
+       (\<lambda> x. if x = home then {''Patient''} else 
+           (if x = hospital then {''Doctor''} else {})) 
      ex_creds' ex_locs"
   
 fixes ex_graph'' :: "igraph"
 defines ex_graph''_def: "ex_graph'' \<equiv> Lgraph 
-     {(room, sphone), (sphone, healthapp), (sphone,bankapp)}
-     (\<lambda> x. if x = room then {''Patient''} else 
-           (if x = sphone then {''Carer''} else {})) 
+     {(home, cloud), (sphone, cloud), (cloud,hospital)}
+       (\<lambda> x. if x = home then {''Patient''} else 
+           (if x = hospital then {''Doctor''} else {})) 
      ex_creds' ex_locs"
 
 fixes ex_graph''' :: "igraph"
  defines ex_graph'''_def: "ex_graph''' \<equiv> Lgraph 
-     {(room, sphone), (sphone, healthapp), (sphone,bankapp)}
-     (\<lambda> x. if x = room then {''Patient''} else 
-              (if x = bankapp then {''Carer''} else {})) 
+     {(home, cloud), (sphone, cloud), (cloud,hospital)}
+       (\<lambda> x. if x = home then {''Patient''} else 
+           (if x = hospital then {''Doctor''} else {})) 
      ex_creds' ex_locs"
  
 fixes local_policies :: "[igraph, location] \<Rightarrow> policy set"
 defines local_policies_def: "local_policies G \<equiv> 
-    (\<lambda> x. if x = room then
+    (\<lambda> x. if x = home then
         {(\<lambda> y. True, {put,get,move,eval})}
           else (if x = sphone then 
              {((\<lambda> y. has G (y, ''PIN'')), {put,get,move,eval})} 
-                else (if x = healthapp then
-                {((\<lambda> y. (\<exists> n. (n  @\<^bsub>G\<^esub> sphone) \<and> Actor n = y)), {put,get,move,eval})}
-                       else (if x = bankapp then
-                {((\<lambda> y. (\<exists> n. ((n  @\<^bsub>G\<^esub> sphone)\<or>(n  @\<^bsub>G\<^esub> bankapp )) \<and> Actor n = y \<and> 
+                else (if x = cloud then
+                {(\<lambda> y. True, {put,get,move,eval})}
+                       else (if x = hospital then
+                {((\<lambda> y. (\<exists> n. (n  @\<^bsub>G\<^esub> hospital) \<and> Actor n = y \<and> 
                            has G (y, ''skey''))), {put,get,move,eval})} else {}))))"
 
+fixes gdpr_scenario :: "infrastructure"
+defines gdpr_scenario_def:
+"gdpr_scenario \<equiv> Infrastructure ex_graph local_policies"
 
-fixes hc_scenario :: "infrastructure"
-defines hc_scenario_def:
-"hc_scenario \<equiv> Infrastructure ex_graph local_policies"
-
-fixes Ihc :: "infrastructure set"
-defines Ihc_def:
-  "Ihc \<equiv> {hc_scenario}"
+fixes Igdpr :: "infrastructure set"
+defines Igdpr_def:
+  "Igdpr \<equiv> {gdpr_scenario}"
 
 (* other states of scenario *)
 
 
 (* First step: Carer is in room with Patient and takes the skey *)
-fixes hc_scenario' :: "infrastructure"
-defines hc_scenario'_def:
-"hc_scenario' \<equiv> Infrastructure ex_graph' local_policies"
+fixes gdpr_scenario' :: "infrastructure"
+defines gdpr_scenario'_def:
+"gdpr_scenario' \<equiv> Infrastructure ex_graph' local_policies"
 
-fixes HC' :: "infrastructure set"
-defines HC'_def:
-  "HC' \<equiv> {hc_scenario'}"
+fixes GDPR' :: "infrastructure set"
+defines GDPR'_def:
+  "GDPR' \<equiv> {gdpr_scenario'}"
 
 
 (* Second step: Carer goes onto sphone and takes the money by eval on bankapp *)
-fixes hc_scenario'' :: "infrastructure"
-defines hc_scenario''_def:
-"hc_scenario'' \<equiv> Infrastructure ex_graph'' local_policies"
+fixes gdpr_scenario'' :: "infrastructure"
+defines gdpr_scenario''_def:
+"gdpr_scenario'' \<equiv> Infrastructure ex_graph'' local_policies"
 
-fixes HC'' :: "infrastructure set"
-defines HC''_def:
-  "HC'' \<equiv> {hc_scenario''}"
+fixes GDPR'' :: "infrastructure set"
+defines GDPR''_def:
+  "GDPR'' \<equiv> {gdpr_scenario''}"
 
 
 (* Third step: Carer goes onto bankapp and can then get money *)
-fixes hc_scenario''' :: "infrastructure"
-defines hc_scenario'''_def:
-"hc_scenario''' \<equiv> Infrastructure ex_graph''' local_policies"
+fixes gdpr_scenario''' :: "infrastructure"
+defines gdpr_scenario'''_def:
+"gdpr_scenario''' \<equiv> Infrastructure ex_graph''' local_policies"
 
-fixes HC''' :: "infrastructure set"
-defines HC'''_def:
-  "HC''' \<equiv> {hc_scenario'''}"
+fixes GDPR''' :: "infrastructure set"
+defines GDPR'''_def:
+  "GDPR''' \<equiv> {gdpr_scenario'''}"
 
 
-fixes hc_states
-defines hc_states_def: "hc_states \<equiv> { I. hc_scenario \<rightarrow>\<^sub>i* I }"
+fixes gdpr_states
+defines gdpr_states_def: "gdpr_states \<equiv> { I. gdpr_scenario \<rightarrow>\<^sub>i* I }"
 
-fixes hc_Kripke
-defines "hc_Kripke \<equiv> Kripke hc_states {hc_scenario}"
+fixes gdpr_Kripke
+defines "gdpr_Kripke \<equiv> Kripke gdpr_states {gdpr_scenario}"
 
-fixes shc 
-defines "shc \<equiv> {x. \<not> (global_policy x ''Carer'')}"  
+fixes sgdpr 
+defines "sgdpr \<equiv> {x. \<not> (global_policy x ''Carer'')}"  
   
 begin
 
-lemma step1: "hc_scenario  \<rightarrow>\<^sub>n hc_scenario'"
-  apply (rule_tac l = room and a' = "''Carer''" and a = "''Patient''" and z = "''skey''" in get)
+(* Base example: Only the Doctor can use data processing in hospital *)  
+lemma gdpr_zero: "gdpr_Kripke \<turnstile> AG {x. (global_policy x ''Doctor'')}"
+  oops
+
+(** GDPR properties  **)    
+(* GDPR one: Owner and listed readers can access*)
+lemma gdpr_one: "h \<in> gdpr_actors \<Longrightarrow> l \<in> gdpr_locations \<Longrightarrow>
+                 Actor h \<in> {owner d} \<union> readers d \<Longrightarrow>
+                 gdpr_Kripke \<turnstile> AG {x. has_access (graphI x) l (Actor h) d}"
+oops
+(* All actors in the infrastructure can delete their data at all times 
+   and at all locations -- this could be moved to the Infrastructure
+   since it holds for all applications *)    
+lemma gdpr_two: "h \<in> gdpr_actors \<Longrightarrow> l \<in> gdpr_locations \<Longrightarrow>
+                 gdpr_Kripke \<turnstile> AG (EX' {x. actor_can_delete x (Actor h) l})"    
+  sorry
+
+theorem GDPR_two: "\<forall> h \<in> gdpr_actors. \<forall> l \<in> gdpr_locations.
+                 gdpr_Kripke \<turnstile> AG (EX' {x. actor_can_delete x (Actor h) l})"    
+  by (simp add: gdpr_two)
+    
+    
+(* GDPR three: Processing preserves ownership in any location *)    
+lemma gdpr_three: "h \<in> gdpr_actors \<Longrightarrow> l \<in> gdpr_locations \<Longrightarrow>
+         owns (Igraph gdpr_scenario) l (Actor h) d \<Longrightarrow>
+         gdpr_Kripke \<turnstile> AG {x. \<forall> l \<in> gdpr_locations. owns (Igraph x) l (Actor h) d }"  
+sorry
+  
+    
+lemma step1: "gdpr_scenario  \<rightarrow>\<^sub>n gdpr_scenario'"
+  apply (rule_tac l = home and a' = "''Doctor''" and a = "''Patient''" and z = "''skey''" in get)
   apply (rule refl)
   apply (simp add: hc_scenario_def atI_def ex_graph_def)+
       apply (simp add: ex_graph_def hc_scenario_def ex_creds_def has_def credentials_def)
@@ -227,15 +259,9 @@ lemma att_hc: "\<turnstile>[\<N>\<^bsub>(Ihc,HC')\<^esub>, \<N>\<^bsub>(HC',HC''
   apply (simp add: att_and)
     apply (rule conjI)
    apply (simp add: Ihc_def HC'_def att_base) 
-   apply (subst state_trans_inst_eq)
-   apply (rule step1)
-  apply (rule conjI)
-   apply (simp add: Ihc_def HC'_def HC''_def att_base) 
-     apply (subst state_trans_inst_eq)
-   apply (rule step2)
-   apply (simp add: Ihc_def HC'_def HC''_def att_base) 
-     apply (subst state_trans_inst_eq)
-by (rule step2)
+    (* instantiation should give that for free 
+    apply (rule step1) *)
+  sorry
     
 
 theorem hc_EF: "hc_Kripke \<turnstile> EF shc"
